compiler/backend/proofs/data_to_word_assignProofScript.sml
@@ -3199,33 +3199,80 @@ Proof
       \\ unabbrev_all_tac \\ fs [IN_domain_adjust_set_inter]))
 QED
 
-Triviality assign_alt_def:
-  assign c secn l dest (MemOp XorByte) args names =
-    case args of [v1;v2] =>
-            (list_Seq [
-                Assign 1 (real_addr c (adjust_var v1));
-                Assign 3 (real_addr c (adjust_var v2));
-                Assign 5 (SmallLsr (Load (Var 3)) (dimindex (:'a) - c.len_size));
-                Assign 1 (Op Add [Var 1; Const bytes_in_word]);
-                Assign 3 (Op Add [Var 3; Const (bytes_in_word:'a word)]);
-                MustTerminate
-                  (Call
-                    (SOME
-                      (adjust_var dest,adjust_set (get_names names),Skip,secn,l))
-                    (SOME XorLoop_location) [1;3;5] NONE);
-                Assign (adjust_var dest) Unit],l + 1)
+Theorem evaluate_XorLoop:
+  ∀a1 a2 l dm m l1 l2 (t1:('a,'c,'ffi) wordSem$state) m1.
+    word_xor_bytes a1 a2 l dm m = SOME m1 ∧ t1.memory = m ∧ t1.mdomain = dm ∧
+    w2n l < t1.clock ∧ good_dimindex (:'a) ∧
+    lookup XorLoop_location t1.code = SOME (4,XorLoop_code) ∧
+    get_var 0 t1 = SOME (Loc l1 l2) ∧
+    get_var 2 t1 = SOME (Word a2) ∧
+    get_var 4 t1 = SOME (Word a1) ∧
+    get_var 6 t1 = SOME (Word l) ⇒
+    ∃ck max_stack.
+      evaluate (XorLoop_code,t1) =
+      (SOME (Result (Loc l1 l2) (Word 2w)),
+       t1 with <| memory := m1; clock := ck; stack_max := max_stack;
+                  locals := LN; locals_size := SOME 0 |>) ∧
+      (max_stack ≠ t1.stack_max ⇒
+       max_stack = OPTION_MAP2 MAX t1.stack_max
+                     (OPTION_MAP2 $+ (stack_size t1.stack)
+                        (lookup XorLoop_location t1.stack_size)))
 Proof
-  cheat
+  ho_match_mp_tac word_xor_bytes_ind \\ rpt gen_tac \\ strip_tac
+  \\ rpt gen_tac
+  \\ once_rewrite_tac [word_xor_bytes_def]
+  \\ simp [SF CONJ_ss,read_word_def]
+  \\ rpt IF_CASES_TAC \\ simp []
+  \\ rpt strip_tac
+  \\ rpt var_eq_tac
+  >~ [‘get_var 6 t1 = SOME (Word 0w)’] >-
+   (fs [wordSemTheory.isWord_exists,theWord_def,wordSemTheory.get_var_def]
+    \\ simp [XorLoop_code_def,eq_eval,wordSemTheory.flush_state_def,list_Seq_def]
+    \\ simp [wordSemTheory.state_component_equality])
+  >~ [‘get_var 6 t1 = SOME (Word l)’,‘l <+ 2w’] >-
+   (fs [wordSemTheory.isWord_exists,theWord_def,wordSemTheory.get_var_def]
+    \\ simp [XorLoop_code_def,eq_eval,wordSemTheory.flush_state_def,list_Seq_def,
+             wordSemTheory.mem_store_def]
+    \\ simp [wordSemTheory.state_component_equality])
+  \\ fs [wordSemTheory.isWord_exists,theWord_def,wordSemTheory.get_var_def,
+        read_word_def] \\ rfs [theWord_def] \\ fs []
+  \\ simp [XorLoop_code_def,eq_eval]
+  (* 4 loads *)
+  \\ ntac 4 $ once_rewrite_tac [list_Seq_def]
+  \\ simp [eq_eval]
+  (* 3 arith *)
+  \\ ntac 3 $ once_rewrite_tac [list_Seq_def]
+  \\ simp [eq_eval]
+  (* 2 stores *)
+  \\ ntac 2 $ once_rewrite_tac [list_Seq_def]
+  \\ simp [eq_eval,wordSemTheory.mem_store_def]
+  (* 2 arith *)
+  \\ ntac 2 $ once_rewrite_tac [list_Seq_def]
+  \\ simp [eq_eval]
+  (* tail call *)
+  \\ simp [eq_eval,list_Seq_def]
+  \\ fs [theWord_def]
+  \\ qmatch_goalsub_abbrev_tac ‘evaluate (XorLoop_code,t2)’
+  \\ last_x_assum $ qspecl_then [‘l1’,‘l2’,‘t2’] mp_tac
+  \\ impl_tac
+  >-
+   (simp [Abbr‘t2’,lookup_insert]
+    \\ Cases_on ‘l’ \\ gvs [good_dimindex_def,dimword_def,WORD_LO]
+    \\ asm_rewrite_tac [GSYM word_sub_def,addressTheory.word_arith_lemma2]
+    \\ simp [dimword_def])
+  \\ strip_tac
+  \\ simp [Abbr‘t2’]
+  \\ qpat_x_assum ‘evaluate _ = _’ kall_tac \\ fs []
+  \\ simp [wordSemTheory.state_component_equality]
 QED
 
 Theorem assign_XorByte:
   op = MemOp XorByte ==> ^assign_thm_goal
 Proof
-
   rpt strip_tac \\ drule0 (evaluate_GiveUp |> GEN_ALL) \\ rw [] \\ fs []
   \\ `t.termdep <> 0` by fs[]
   \\ rpt_drule0 state_rel_cut_IMP \\ strip_tac
-  \\ imp_res_tac get_vars_IMP_LENGTH \\ fs [assign_alt_def] \\ rw []
+  \\ imp_res_tac get_vars_IMP_LENGTH \\ fs [assign_def] \\ rw []
   \\ fs [do_app,allowed_op_def]
   \\ gvs [AllCaseEqs()]
   \\ gvs [LENGTH_EQ_NUM_compute]
@@ -3271,441 +3318,85 @@ Proof
   \\ ntac 2 $ once_rewrite_tac [list_Seq_def]
   \\ simp [eq_eval,get_names_def]
   (* call *)
-
-  \\  cheat (* XorByte
-
-  \\ fs [wordSemTheory.evaluate_def,wordSemTheory.add_ret_loc_def,
-         wordSemTheory.bad_dest_args_def,wordSemTheory.find_code_def,
-         get_names_def]
-  \\ rpt_drule0 state_rel_get_vars_IMP \\ strip_tac \\ fs []
-  \\ `lookup XorLoop_location t.code = SOME (4,XorLoop_code c)` by cheat (*
-       (fs [state_rel_def,code_rel_def,stubs_def] \\ NO_TAC) \\ fs [] *)
-  \\ fs [cut_state_opt_def,cut_state_def]
-  \\ pop_assum kall_tac
-  \\ rename1 `state_rel c l1 l2 s1 t [] locs`
-  \\ Cases_on `dataSem$cut_env x'' s.locals` \\ fs []
-  \\ clean_tac \\ fs []
-  \\ qabbrev_tac `s1 = s with locals := x`
-  \\ `?y. cut_env (adjust_set x'') t.locals = SOME y` by
-       (match_mp_tac (GEN_ALL cut_env_IMP_cut_env) \\ fs []
-        \\ metis_tac []) \\ fs []
-  \\ fs [LENGTH_EQ_5] \\ rveq
-  \\ qpat_assum `state_rel c l1 l2 s1 t [] locs` mp_tac
-  \\ simp_tac std_ss [Once state_rel_thm] \\ strip_tac \\ fs []
-  \\ full_simp_tac std_ss [GSYM APPEND_ASSOC]
-  \\ qpat_x_assum `get_vars _ x = _` mp_tac
-  \\ `x = s1.locals` by fs [Abbr`s1`]
-  \\ pop_assum (fn th => rewrite_tac [th]) \\ strip_tac
-  \\ rpt_drule0 memory_rel_lookup_var_IMP \\ strip_tac
-  \\ fs []
-  \\ `s.refs = s1.refs`     by rw [Abbr `s1`]
-  \\ `s.space = s1.space`   by rw [Abbr `s1`]
-  \\ `s.global = s1.global` by rw [Abbr `s1`]
-  \\ `s.stack  = s1.stack`  by rw [Abbr `s1`]
-  \\ `?xp yp len_n.
-        srcoff = &xp /\ xp < dimword (:'a) DIV 8 /\
-        dstoff = &yp /\ yp < dimword (:'a) DIV 8 /\
-        le = &len_n /\ len_n < dimword (:'a) DIV 8` by
-   (fs [semanticPrimitivesTheory.copy_array_def,not_less_zero_int_eq]
-    \\ rveq \\ fs [NOT_LESS,integerTheory.INT_ADD,integerTheory.INT_ABS_NUM]
-    \\ rpt_drule0 memory_rel_ByteArray_IMP
-    \\ ntac 3 (drule0 memory_rel_tl \\ pop_assum kall_tac \\ strip_tac)
-    \\ rpt_drule0 memory_rel_ByteArray_IMP
-    \\ fs [good_dimindex_def,dimword_def]
-    \\ rpt strip_tac \\ fs [])
-  \\ rveq \\ fs []
-  \\ `∃w. a3 = Word w ∧ w ⋙ 2 = n2w len_n` by
-        (rpt_drule0 memory_rel_get_num \\ metis_tac [])
-  \\ rveq \\ fs [] \\ ntac 2 (pop_assum mp_tac)
-  \\ `∃w. a5 = Word w ∧ w ⋙ 2 = n2w yp` by
-        (rpt_drule0 memory_rel_get_num \\ metis_tac [])
-  \\ rveq \\ fs [] \\ ntac 2 (pop_assum mp_tac)
-  \\ `∃w. a2 = Word w ∧ w ⋙ 2 = n2w xp` by
-        (rpt_drule0 memory_rel_get_num \\ metis_tac [])
-  \\ rveq \\ fs [] \\ rpt strip_tac
-  \\ fs [ByteCopy_code_def,wordSemTheory.call_env_def,fromList2_def]
-  \\ qpat_x_assum `wordSem$get_vars _ _ = _` kall_tac
-  \\ once_rewrite_tac [list_Seq_def] \\ eval_tac
-  \\ once_rewrite_tac [word_exp_set_var_ShiftVar_lemma] \\ fs [eq_eval]
-  \\ once_rewrite_tac [list_Seq_def] \\ eval_tac
-  \\ once_rewrite_tac [word_exp_set_var_ShiftVar_lemma] \\ fs [eq_eval]
-  \\ once_rewrite_tac [list_Seq_def] \\ eval_tac
-  \\ once_rewrite_tac [word_exp_set_var_ShiftVar_lemma] \\ fs [eq_eval]
-  \\ once_rewrite_tac [list_Seq_def] \\ fs [Unit_def] \\ eval_tac
-  \\ `?wa1 addr1. a1 = Word wa1 /\ get_real_addr c t.store wa1 = SOME addr1`
-          by (rpt_drule0 memory_rel_ByteArray_IMP \\ strip_tac \\ fs [])
-  \\ `?wa2 addr2. a4 = Word wa2 /\ get_real_addr c t.store wa2 = SOME addr2`
-          by (ntac 3 (drule0 memory_rel_tl \\ strip_tac)
-              \\ rpt_drule0 memory_rel_ByteArray_IMP \\ strip_tac \\ fs [])
-  \\ rveq \\ fs []
-  \\ qmatch_goalsub_abbrev_tac `wordSem$evaluate (_,t7)`
-  \\ `get_var 2 t7 = SOME (Word wa1)` by
-      (unabbrev_all_tac \\ fs [wordSemTheory.get_var_def,lookup_insert])
-  \\ once_rewrite_tac [list_Seq_def] \\ eval_tac
-  \\ `t7.store = t.store` by (unabbrev_all_tac \\ fs [push_env_store])
-  \\ rpt_drule0 get_var_get_real_addr_lemma
-  \\ disch_then kall_tac
-  \\ qunabbrev_tac `t7` \\ fs [eq_eval]
-  \\ qmatch_goalsub_abbrev_tac `wordSem$evaluate (_,t7)`
-  \\ `get_var 8 t7 = SOME (Word wa2)` by
-      (unabbrev_all_tac \\ fs [wordSemTheory.get_var_def,lookup_insert])
-  \\ once_rewrite_tac [list_Seq_def] \\ eval_tac
-  \\ `t7.store = t.store` by (unabbrev_all_tac \\ fs [push_env_store])
-  \\ rpt_drule0 get_var_get_real_addr_lemma
-  \\ disch_then kall_tac
-  \\ qunabbrev_tac `t7` \\ fs [eq_eval]
-  \\ pop_assum kall_tac \\ clean_tac
+  \\ fs [cut_state_opt_def,cut_state_def,CaseEq"option"]
+  \\ qabbrev_tac `s1 = s with locals := env` \\ var_eq_tac
+  \\ drule_all cut_env_IMP_cut_env \\ strip_tac
   \\ once_rewrite_tac [list_Seq_def]
-  \\ Cases_on `src = dst` (* alias case *) \\ rveq
-  THEN1
-   (`wa2 = wa1` by
-     (drule0 memory_rel_swap \\ strip_tac
-      \\ drule0 memory_rel_tl \\ strip_tac
-      \\ drule0 memory_rel_swap \\ strip_tac
-      \\ drule0 memory_rel_tl \\ strip_tac
-      \\ drule memory_rel_RefPtr_EQ_IMP
-      \\ gvs [])
-    \\ fs [] \\ rveq
-    \\ `memory_rel c t.be (THE s1.tstamps) s1.refs s1.space t.store t.memory t.mdomain
-         ((RefPtr dst_b dst,Word wa1)::
-            (join_env s1.locals
-               (toAList (inter t.locals (adjust_set s1.locals))) ++
-             [(the_global s1.global,t.store ' Globals)] ++
-             flat s1.stack t.stack))` by
-     (first_x_assum (fn th => mp_tac th THEN match_mp_tac memory_rel_rearrange)
-      \\ fs [] \\ rw [] \\ fs [])
-    \\ rpt_drule0 word_copy_array_alias_thm
-    \\ strip_tac
-    \\ qpat_x_assum `_ = SOME m1` mp_tac
-    \\ fs [word_copy_array_def,GSYM WORD_NOT_LOWER]
-    \\ IF_CASES_TAC \\ fs [] \\ strip_tac
-    THEN1
-     (once_rewrite_tac [wordSemTheory.evaluate_def] \\ eval_tac
-      \\ fs [wordSemTheory.get_var_def,wordSemTheory.get_var_imm_def,
-             lookup_insert,asmTheory.word_cmp_def,wordSemTheory.bad_dest_args_def,
-             wordSemTheory.find_code_def,eq_eval,push_env_code]
-      \\ `lookup ByteCopyAdd_location t.code = SOME (5,ByteCopyAdd_code)` by
-           (fs [state_rel_def,code_rel_def,stubs_def] \\ NO_TAC) \\ fs []
-      \\ fs []
-      \\ assume_tac CopyByteAdd_thm \\ SEP_I_TAC "evaluate"
-      \\ pop_assum drule0 \\ fs [eq_eval]
-      \\ impl_tac THEN1
-       (fs [push_env_store]
-        \\ fs [good_dimindex_def,dimword_def] \\ rfs []
-        \\ match_mp_tac LESS_EQ_TRANS
-        \\ qexists_tac `dimword (:'a)` \\ conj_tac
-        \\ TRY (fs [dimword_def,DIV_LE_X] \\ NO_TAC)
-        \\ `2 <= dimword (:'a)` by fs [dimword_def]
-        \\ fs [wordSemTheory.MustTerminate_limit_def])
-      \\ fs [] \\ disch_then kall_tac
-      \\ fs [wordSemTheory.pop_env_def,wordSemTheory.push_env_def]
-      \\ Cases_on `env_to_list y t.permute` \\ fs []
-      \\ `domain (fromAList q) = domain y` by
-          (drule0 env_to_list_lookup_equiv
-           \\ fs [EXTENSION,domain_lookup,lookup_fromAList]) \\ fs []
-      \\ fs [state_rel_thm,lookup_insert,lookup_fromAList,adjust_var_11]
-      \\ drule0 env_to_list_lookup_equiv \\ fs [] \\ strip_tac
-      \\ conj_tac THEN1
-       (drule0 env_to_list_lookup_equiv
-        \\ fs [lookup_insert,lookup_fromAList]
-        \\ fs [wordSemTheory.cut_env_def] \\ rveq
-        \\ pop_assum imp_res_tac
-        \\ fs [cut_state_def,cut_env_def] \\ rveq
-        \\ simp [lookup_inter_alt,ZERO_IN_adjust_set])
-      \\ conj_tac THEN1
-        (drule0 env_to_list_lookup_equiv
-         \\ fs [lookup_insert,lookup_fromAList,adjust_var_11]
-         \\ rw [] \\ rw [] \\ fs [] \\ unabbrev_all_tac \\ fs []
-         \\ fs [wordSemTheory.cut_env_def] \\ rveq
-         \\ qpat_x_assum `!x._` imp_res_tac
-         \\ fs [cut_state_def,cut_env_def] \\ rveq
-         \\ Cases_on `domain x'' ⊆ domain s.locals` \\ fs [] \\ rveq
-         \\ fs [] \\ fs [lookup_inter_alt,adjust_var_IN_adjust_set]
-         \\ rw [] \\ fs [])
-      \\ conj_tac THEN1
-         (simp[stack_size_eq,option_le_max_right,AC option_add_comm option_add_assoc])
-      \\ conj_tac THEN1
-         (imp_res_tac stack_rel_IMP_size_of_stack >>
-          rfs[stack_size_eq,option_le_max,option_le_max_right,
-              AC option_add_comm option_add_assoc,option_le_eq_eqns,
-              option_map2_max_add,option_le_add])
-      \\ simp [FAPPLY_FUPDATE_THM]
-      \\ full_simp_tac std_ss [GSYM APPEND_ASSOC]
-      \\ match_mp_tac memory_rel_insert \\ fs []
-      \\ match_mp_tac memory_rel_Unit
-      \\ drule0 memory_rel_tl \\ fs []
-      \\ match_mp_tac quotientTheory.EQ_IMPLIES
-      \\ `s1.tstamps = s.tstamps` by fs [Abbr `s1`] \\ fs []
-      \\ AP_TERM_TAC \\ fs []
-      \\ fs [wordSemTheory.cut_env_def] \\ rveq
-      \\ qpat_x_assum `!x._` imp_res_tac
-      \\ fs [cut_state_def,cut_env_def] \\ rveq
-      \\ Cases_on `domain x'' ⊆ domain s.locals` \\ fs [] \\ rveq \\ fs []
-      \\ fs [join_env_def]
-      \\ match_mp_tac (METIS_PROVE [] ``f x = g x /\ x = y ==> f x = g y``)
-      \\ conj_tac THEN1
-       (fs [MAP_EQ_f,FORALL_PROD,MEM_FILTER,MEM_toAList,lookup_inter_alt]
-        \\ rpt strip_tac \\ rw [] \\ sg `F` \\ fs []
-        \\ pop_assum mp_tac \\ fs [Abbr `nms`,domain_list_insert])
-      \\ AP_TERM_TAC \\ AP_TERM_TAC
-      \\ fs [spt_eq_thm,lookup_inter_alt]
-      \\ rw [] \\ fs []
-      \\ drule0 env_to_list_lookup_equiv
-      \\ fs [lookup_insert,lookup_fromAList,adjust_var_11]
-      \\ rpt strip_tac \\ fs []
-      \\ fs [lookup_inter_alt] \\ rw []
-      \\ sg `F` \\ fs [] \\ pop_assum mp_tac \\ simp []
-      \\ unabbrev_all_tac \\ fs [IN_domain_adjust_set_inter])
-    THEN1
-     (rewrite_tac [wordSemTheory.evaluate_def,list_Seq_def] \\ eval_tac
-      \\ fs [wordSemTheory.get_var_def,wordSemTheory.get_var_imm_def,
-             lookup_insert,asmTheory.word_cmp_def,wordSemTheory.bad_dest_args_def,
-             wordSemTheory.find_code_def,eq_eval,push_env_code]
-      \\ `lookup ByteCopySub_location t.code = SOME (5,ByteCopySub_code)` by
-           (fs [state_rel_def,code_rel_def,stubs_def] \\ NO_TAC) \\ fs []
-      \\ fs []
-      \\ assume_tac CopyByteSub_thm \\ SEP_I_TAC "evaluate"
-      \\ pop_assum drule0 \\ fs [eq_eval]
-      \\ impl_tac THEN1
-       (fs [push_env_store]
-        \\ fs [good_dimindex_def,dimword_def] \\ rfs []
-        \\ match_mp_tac LESS_EQ_TRANS
-        \\ qexists_tac `dimword (:'a)` \\ conj_tac
-        \\ TRY (fs [dimword_def,DIV_LE_X] \\ NO_TAC)
-        \\ `2 <= dimword (:'a)` by fs [dimword_def]
-        \\ fs [wordSemTheory.MustTerminate_limit_def])
-      \\ fs [] \\ disch_then kall_tac
-      \\ fs [wordSemTheory.pop_env_def,wordSemTheory.push_env_def]
-      \\ Cases_on `env_to_list y t.permute` \\ fs []
-      \\ `domain (fromAList q) = domain y` by
-          (drule0 env_to_list_lookup_equiv
-           \\ fs [EXTENSION,domain_lookup,lookup_fromAList]) \\ fs []
-      \\ fs [state_rel_thm,lookup_insert,lookup_fromAList,adjust_var_11]
-      \\ drule0 env_to_list_lookup_equiv \\ fs [] \\ strip_tac
-      \\ conj_tac THEN1
-       (drule0 env_to_list_lookup_equiv
-        \\ fs [lookup_insert,lookup_fromAList]
-        \\ fs [wordSemTheory.cut_env_def] \\ rveq
-        \\ qpat_x_assum `!x._` imp_res_tac
-        \\ fs [cut_state_def,cut_env_def] \\ rveq
-        \\ simp [lookup_inter_alt,ZERO_IN_adjust_set])
-      \\ conj_tac THEN1
-        (drule0 env_to_list_lookup_equiv
-         \\ fs [lookup_insert,lookup_fromAList,adjust_var_11]
-         \\ rw [] \\ rw [] \\ fs [] \\ unabbrev_all_tac \\ fs []
-         \\ fs [wordSemTheory.cut_env_def] \\ rveq
-         \\ qpat_x_assum `!x._` imp_res_tac
-         \\ fs [cut_state_def,cut_env_def] \\ rveq
-         \\ Cases_on `domain x'' ⊆ domain s.locals` \\ fs [] \\ rveq
-         \\ fs [] \\ fs [lookup_inter_alt,adjust_var_IN_adjust_set]
-         \\ rw [] \\ fs [])
-      \\ conj_tac THEN1
-         (simp[stack_size_eq,option_le_max_right,AC option_add_comm option_add_assoc])
-      \\ conj_tac THEN1
-         (imp_res_tac stack_rel_IMP_size_of_stack >>
-          rfs[stack_size_eq,option_le_max,option_le_max_right,
-              AC option_add_comm option_add_assoc,option_le_eq_eqns,
-              option_map2_max_add,option_le_add])
-      \\ simp [FAPPLY_FUPDATE_THM]
-      \\ full_simp_tac std_ss [GSYM APPEND_ASSOC]
-      \\ match_mp_tac memory_rel_insert \\ fs []
-      \\ match_mp_tac memory_rel_Unit
-      \\ drule0 memory_rel_tl \\ fs []
-      \\ match_mp_tac quotientTheory.EQ_IMPLIES
-      \\ `s1.tstamps = s.tstamps` by fs [Abbr `s1`] \\ fs []
-      \\ AP_TERM_TAC \\ fs []
-      \\ fs [wordSemTheory.cut_env_def] \\ rveq
-      \\ qpat_x_assum `!x._` imp_res_tac
-      \\ fs [cut_state_def,cut_env_def] \\ rveq
-      \\ Cases_on `domain x'' ⊆ domain s.locals` \\ fs [] \\ rveq \\ fs []
-      \\ fs [join_env_def]
-      \\ match_mp_tac (METIS_PROVE [] ``f x = g x /\ x = y ==> f x = g y``)
-      \\ conj_tac THEN1
-       (fs [MAP_EQ_f,FORALL_PROD,MEM_FILTER,MEM_toAList,lookup_inter_alt]
-        \\ rpt strip_tac \\ rw [] \\ sg `F` \\ fs []
-        \\ pop_assum mp_tac \\ fs [Abbr `nms`,domain_list_insert])
-      \\ AP_TERM_TAC \\ AP_TERM_TAC
-      \\ fs [spt_eq_thm,lookup_inter_alt]
-      \\ rw [] \\ fs []
-      \\ drule0 env_to_list_lookup_equiv
-      \\ fs [lookup_insert,lookup_fromAList,adjust_var_11]
-      \\ rpt strip_tac \\ fs []
-      \\ fs [lookup_inter_alt] \\ rw []
-      \\ sg `F` \\ fs [] \\ pop_assum mp_tac \\ simp []
-      \\ unabbrev_all_tac \\ fs [IN_domain_adjust_set_inter]))
-  THEN1
-   (`memory_rel c t.be (THE s1.tstamps) s1.refs s1.space t.store t.memory t.mdomain
-         ((RefPtr src_b src,Word wa1)::(RefPtr dst_b dst,Word wa2)::
-            (join_env s1.locals
-               (toAList (inter t.locals (adjust_set s1.locals))) ++
-             [(the_global s1.global,t.store ' Globals)] ++
-             flat s1.stack t.stack))` by
-     (first_x_assum (fn th => mp_tac th THEN match_mp_tac memory_rel_rearrange)
-      \\ fs [] \\ rw [] \\ fs [])
-    \\ rpt_drule0 word_copy_array_thm
-    \\ strip_tac
-    \\ qpat_x_assum `_ = SOME m1` mp_tac
-    \\ fs [word_copy_array_def,GSYM WORD_NOT_LOWER]
-    \\ IF_CASES_TAC \\ fs [] \\ strip_tac
-    THEN1
-     (once_rewrite_tac [wordSemTheory.evaluate_def] \\ eval_tac
-      \\ fs [wordSemTheory.get_var_def,wordSemTheory.get_var_imm_def,
-             lookup_insert,asmTheory.word_cmp_def,wordSemTheory.bad_dest_args_def,
-             wordSemTheory.find_code_def,eq_eval,push_env_code]
-      \\ `lookup ByteCopyAdd_location t.code = SOME (5,ByteCopyAdd_code)` by
-           (fs [state_rel_def,code_rel_def,stubs_def] \\ NO_TAC) \\ fs []
-      \\ fs []
-      \\ assume_tac CopyByteAdd_thm \\ SEP_I_TAC "evaluate"
-      \\ pop_assum drule0 \\ fs [eq_eval]
-      \\ impl_tac THEN1
-       (fs [push_env_store]
-        \\ fs [good_dimindex_def,dimword_def] \\ rfs []
-        \\ match_mp_tac LESS_EQ_TRANS
-        \\ qexists_tac `dimword (:'a)` \\ conj_tac
-        \\ TRY (fs [dimword_def,DIV_LE_X] \\ NO_TAC)
-        \\ `2 <= dimword (:'a)` by fs [dimword_def]
-        \\ fs [wordSemTheory.MustTerminate_limit_def])
-      \\ fs [] \\ disch_then kall_tac
-      \\ fs [wordSemTheory.pop_env_def,wordSemTheory.push_env_def]
-      \\ Cases_on `env_to_list y t.permute` \\ fs []
-      \\ `domain (fromAList q) = domain y` by
-          (drule0 env_to_list_lookup_equiv
-           \\ fs [EXTENSION,domain_lookup,lookup_fromAList]) \\ fs []
-      \\ fs [state_rel_thm,lookup_insert,lookup_fromAList,adjust_var_11]
-      \\ drule0 env_to_list_lookup_equiv \\ fs [] \\ strip_tac
-      \\ conj_tac THEN1
-       (drule0 env_to_list_lookup_equiv
-        \\ fs [lookup_insert,lookup_fromAList]
-        \\ fs [wordSemTheory.cut_env_def] \\ rveq
-        \\ qpat_x_assum `!x._` imp_res_tac
-        \\ fs [cut_state_def,cut_env_def] \\ rveq
-        \\ simp [lookup_inter_alt,ZERO_IN_adjust_set])
-      \\ conj_tac THEN1
-        (drule0 env_to_list_lookup_equiv
-         \\ fs [lookup_insert,lookup_fromAList,adjust_var_11]
-         \\ rw [] \\ rw [] \\ fs [] \\ unabbrev_all_tac \\ fs []
-         \\ fs [wordSemTheory.cut_env_def] \\ rveq
-         \\ qpat_x_assum `!x._` imp_res_tac
-         \\ fs [cut_state_def,cut_env_def] \\ rveq
-         \\ Cases_on `domain x'' ⊆ domain s.locals` \\ fs [] \\ rveq
-         \\ fs [] \\ fs [lookup_inter_alt,adjust_var_IN_adjust_set]
-         \\ rw [] \\ fs [])
-      \\ conj_tac THEN1
-         (simp[stack_size_eq,option_le_max_right,AC option_add_comm option_add_assoc])
-      \\ conj_tac THEN1
-         (imp_res_tac stack_rel_IMP_size_of_stack >>
-          rfs[stack_size_eq,option_le_max,option_le_max_right,
-              AC option_add_comm option_add_assoc,option_le_eq_eqns,
-              option_map2_max_add,option_le_add])
-      \\ simp [FAPPLY_FUPDATE_THM]
-      \\ full_simp_tac std_ss [GSYM APPEND_ASSOC]
-      \\ match_mp_tac memory_rel_insert \\ fs []
-      \\ match_mp_tac memory_rel_Unit
-      \\ drule0 memory_rel_tl \\ fs [] \\ strip_tac
-      \\ drule0 memory_rel_tl \\ fs [] \\ pop_assum kall_tac
-      \\ match_mp_tac quotientTheory.EQ_IMPLIES
-      \\ `s1.tstamps = s.tstamps` by fs [Abbr `s1`] \\ fs []
-      \\ AP_TERM_TAC \\ fs []
-      \\ fs [wordSemTheory.cut_env_def] \\ rveq
-      \\ qpat_x_assum `!x._` imp_res_tac
-      \\ fs [cut_state_def,cut_env_def] \\ rveq
-      \\ Cases_on `domain x'' ⊆ domain s.locals` \\ fs [] \\ rveq \\ fs []
-      \\ fs [join_env_def]
-      \\ match_mp_tac (METIS_PROVE [] ``f x = g x /\ x = y ==> f x = g y``)
-      \\ conj_tac THEN1
-       (fs [MAP_EQ_f,FORALL_PROD,MEM_FILTER,MEM_toAList,lookup_inter_alt]
-        \\ rpt strip_tac \\ rw [] \\ sg `F` \\ fs []
-        \\ pop_assum mp_tac \\ fs [Abbr `nms`,domain_list_insert])
-      \\ AP_TERM_TAC \\ AP_TERM_TAC
-      \\ fs [spt_eq_thm,lookup_inter_alt]
-      \\ rw [] \\ fs []
-      \\ drule0 env_to_list_lookup_equiv
-      \\ fs [lookup_insert,lookup_fromAList,adjust_var_11]
-      \\ rpt strip_tac \\ fs []
-      \\ fs [lookup_inter_alt] \\ rw []
-      \\ sg `F` \\ fs [] \\ pop_assum mp_tac \\ simp []
-      \\ unabbrev_all_tac \\ fs [IN_domain_adjust_set_inter])
-    THEN1
-     (rewrite_tac [wordSemTheory.evaluate_def,list_Seq_def] \\ eval_tac
-      \\ fs [wordSemTheory.get_var_def,wordSemTheory.get_var_imm_def,
-             lookup_insert,asmTheory.word_cmp_def,wordSemTheory.bad_dest_args_def,
-             wordSemTheory.find_code_def,eq_eval,push_env_code]
-      \\ `lookup ByteCopySub_location t.code = SOME (5,ByteCopySub_code)` by
-           (fs [state_rel_def,code_rel_def,stubs_def] \\ NO_TAC) \\ fs []
-      \\ fs []
-      \\ assume_tac CopyByteSub_thm \\ SEP_I_TAC "evaluate"
-      \\ pop_assum drule0 \\ fs [eq_eval]
-      \\ impl_tac THEN1
-       (fs [push_env_store]
-        \\ fs [good_dimindex_def,dimword_def] \\ rfs []
-        \\ match_mp_tac LESS_EQ_TRANS
-        \\ qexists_tac `dimword (:'a)` \\ conj_tac
-        \\ TRY (fs [dimword_def,DIV_LE_X] \\ NO_TAC)
-        \\ `2 <= dimword (:'a)` by fs [dimword_def]
-        \\ fs [wordSemTheory.MustTerminate_limit_def])
-      \\ fs [] \\ disch_then kall_tac
-      \\ fs [wordSemTheory.pop_env_def,wordSemTheory.push_env_def]
-      \\ Cases_on `env_to_list y t.permute` \\ fs []
-      \\ `domain (fromAList q) = domain y` by
-          (drule0 env_to_list_lookup_equiv
-           \\ fs [EXTENSION,domain_lookup,lookup_fromAList]) \\ fs []
-      \\ fs [state_rel_thm,lookup_insert,lookup_fromAList,adjust_var_11]
-      \\ drule0 env_to_list_lookup_equiv \\ fs [] \\ strip_tac
-      \\ conj_tac THEN1
-       (drule0 env_to_list_lookup_equiv
-        \\ fs [lookup_insert,lookup_fromAList]
-        \\ fs [wordSemTheory.cut_env_def] \\ rveq
-        \\ qpat_x_assum `!x._` imp_res_tac
-        \\ fs [cut_state_def,cut_env_def] \\ rveq
-        \\ simp [lookup_inter_alt,ZERO_IN_adjust_set])
-      \\ conj_tac THEN1
-        (drule0 env_to_list_lookup_equiv
-         \\ fs [lookup_insert,lookup_fromAList,adjust_var_11]
-         \\ rw [] \\ rw [] \\ fs [] \\ unabbrev_all_tac \\ fs []
-         \\ fs [wordSemTheory.cut_env_def] \\ rveq
-         \\ qpat_x_assum `!x._` imp_res_tac
-         \\ fs [cut_state_def,cut_env_def] \\ rveq
-         \\ Cases_on `domain x'' ⊆ domain s.locals` \\ fs [] \\ rveq
-         \\ fs [] \\ fs [lookup_inter_alt,adjust_var_IN_adjust_set]
-         \\ rw [] \\ fs [])
-      \\ conj_tac THEN1
-         (simp[stack_size_eq,option_le_max_right,AC option_add_comm option_add_assoc])
-      \\ conj_tac THEN1
-         (imp_res_tac stack_rel_IMP_size_of_stack >>
-          rfs[stack_size_eq,option_le_max,option_le_max_right,
-              AC option_add_comm option_add_assoc,option_le_eq_eqns,
-              option_map2_max_add,option_le_add])
-      \\ simp [FAPPLY_FUPDATE_THM]
-      \\ full_simp_tac std_ss [GSYM APPEND_ASSOC]
-      \\ match_mp_tac memory_rel_insert \\ fs []
-      \\ match_mp_tac memory_rel_Unit
-      \\ drule0 memory_rel_tl \\ fs [] \\ strip_tac
-      \\ drule0 memory_rel_tl \\ fs [] \\ pop_assum kall_tac
-      \\ match_mp_tac quotientTheory.EQ_IMPLIES
-      \\ `s1.tstamps = s.tstamps` by fs [Abbr `s1`] \\ fs []
-      \\ AP_TERM_TAC \\ fs []
-      \\ fs [wordSemTheory.cut_env_def] \\ rveq
-      \\ qpat_x_assum `!x._` imp_res_tac
-      \\ fs [cut_state_def,cut_env_def] \\ rveq
-      \\ Cases_on `domain x'' ⊆ domain s.locals` \\ fs [] \\ rveq \\ fs []
-      \\ fs [join_env_def]
-      \\ match_mp_tac (METIS_PROVE [] ``f x = g x /\ x = y ==> f x = g y``)
-      \\ conj_tac THEN1
-       (fs [MAP_EQ_f,FORALL_PROD,MEM_FILTER,MEM_toAList,lookup_inter_alt]
-        \\ rpt strip_tac \\ rw [] \\ sg `F` \\ fs []
-        \\ pop_assum mp_tac \\ fs [Abbr `nms`,domain_list_insert])
-      \\ AP_TERM_TAC \\ AP_TERM_TAC
-      \\ fs [spt_eq_thm,lookup_inter_alt]
-      \\ rw [] \\ fs []
-      \\ drule0 env_to_list_lookup_equiv
-      \\ fs [lookup_insert,lookup_fromAList,adjust_var_11]
-      \\ rpt strip_tac \\ fs []
-      \\ fs [lookup_inter_alt] \\ rw []
-      \\ sg `F` \\ fs [] \\ pop_assum mp_tac \\ simp []
-      \\ unabbrev_all_tac \\ fs [IN_domain_adjust_set_inter]))
-
-  *)
-
+  \\ `lookup XorLoop_location t.code = SOME (4,XorLoop_code c)` by
+    fs [state_rel_def,code_rel_def,stubs_def]
+  \\ simp [eq_eval,cut_env_adjust_set_insert_ODD]
+  \\ Cases_on ‘env_to_list y t.permute’
+  \\ simp [wordSemTheory.push_env_def]
+  \\ qmatch_goalsub_abbrev_tac ‘evaluate (XorLoop_code,t1)’
+  \\ rename [‘insert 0 (Loc rl1 rl2) LN’]
+  \\ drule evaluate_XorLoop
+  \\ disch_then $ qspecl_then [‘rl1’,‘rl2’,‘t1’] mp_tac
+  \\ impl_tac
+  >-
+   (simp [Abbr‘t1’,wordSemTheory.get_var_def,lookup_insert]
+    \\ irule LESS_LESS_EQ_TRANS
+    \\ irule_at Any w2n_lt
+    \\ rewrite_tac [wordSemTheory.MustTerminate_limit_def]
+    \\ ‘dimword (:α) < 2 * dimword (:α)’ by gvs [good_dimindex_def,dimword_def]
+    \\ decide_tac)
+  \\ qpat_x_assum ‘lookup XorLoop_location _ = _’ kall_tac
+  \\ strip_tac \\ simp []
+  \\ simp [Abbr‘t1’,wordSemTheory.pop_env_def]
+  \\ reverse $ IF_CASES_TAC
+  >-
+   (qsuff_tac ‘F’ >- rewrite_tac []
+    \\ drule env_to_list_lookup_equiv
+    \\ fs [EXTENSION,domain_lookup,lookup_fromAList]
+    \\ fs[GSYM IS_SOME_EXISTS]
+    \\ CCONTR_TAC \\ fs [])
+  \\ simp []
+  (* final part: proving state_rel *)
+  \\ simp [list_Seq_def,eq_eval,data_to_wordTheory.Unit_def]
+  \\ ntac 2 $ pop_assum kall_tac
+  \\ qpat_x_assum ‘state_rel c l1 l2 s1 t [] locs’ mp_tac
+  \\ simp [state_rel_thm,dataSemTheory.set_var_def,lookup_insert]
+  \\ strip_tac \\ pop_assum kall_tac
+  \\ conj_tac >-
+   (gvs [wordSemTheory.cut_env_def]
+    \\ drule env_to_list_lookup_equiv
+    \\ fs [EXTENSION,domain_lookup,lookup_fromAList]
+    \\ strip_tac \\ fs [lookup_inter,lookup_0_adjust_set])
+  \\ conj_tac >-
+   (rewrite_tac [adjust_var_11] \\ rw []
+    \\ gvs [wordSemTheory.cut_env_def]
+    \\ drule env_to_list_lookup_equiv
+    \\ simp [lookup_fromAList]
+    \\ fs [IS_SOME_lookup_domain,domain_inter]
+    \\ rw [adjust_var_IN_adjust_set]
+    \\ fs [dataSemTheory.cut_env_def]
+    \\ qunabbrev_tac ‘s1’
+    \\ rpt var_eq_tac
+    \\ fs [domain_inter])
+  \\ conj_tac >- cheat
+  \\ conj_tac >- cheat
+  (* memory_rel *)
+  \\ once_rewrite_tac [insert_insert] \\ rewrite_tac []
+  \\ rewrite_tac [GSYM APPEND_ASSOC,APPEND]
+  \\ irule memory_rel_insert \\ rewrite_tac [APPEND]
+  \\ irule memory_rel_Unit \\ asm_rewrite_tac []
+  \\ qpat_x_assum ‘_ t.mdomain _’ mp_tac
+  \\ match_mp_tac memory_rel_rearrange
+  \\ simp [SF DNF_ss]
+  \\ qsuff_tac ‘inter (fromAList q) (adjust_set s1.locals) =
+                inter t.locals (adjust_set s1.locals)’
+  >- asm_simp_tac std_ss []
+  \\ simp [lookup_inter_alt]
+  \\ qunabbrev_tac ‘s1’ \\ simp []
+  \\ qx_gen_tac ‘nm’
+  \\ IF_CASES_TAC \\ rewrite_tac []
+  \\ drule0 env_to_list_lookup_equiv
+  \\ fs [lookup_insert,lookup_fromAList,adjust_var_11]
+  \\ fs [wordSemTheory.cut_env_def]
+  \\ fs [dataSemTheory.cut_env_def]
+  \\ rpt var_eq_tac
+  \\ simp [lookup_inter_alt]
+  \\ rpt strip_tac
+  \\ fs [IN_domain_adjust_set_inter]
 QED
 
 Triviality evaluate_AppendMainLoop_code:
